James C - migrated linearize to a generic finite map fold

FiniteMap.thy
@@ -12,30 +12,36 @@ fun domain_distinct :: "'a \<leadsto> 'b \<Rightarrow> bool" where
   "domain_distinct [] = True"
 | "domain_distinct ((a, b) # ab) = (domain_distinct ab \<and> a \<notin> dom (lookup ab))"
 
-function linearize :: "('a \<rightharpoonup> 'b) \<Rightarrow> 'a \<leadsto> 'b" where
-  "\<not> finite (dom f) \<Longrightarrow> linearize f = undefined"
-| "finite (dom f) \<Longrightarrow> card (dom f) = 0 \<Longrightarrow> linearize f = []"
-| "finite (dom f) \<Longrightarrow> card (dom f) \<noteq> 0 \<Longrightarrow> linearize f = (
-    let x = SOME x. x \<in> dom f
-    in (x, the (f x)) # linearize (f(x := None)))"
+function finite_map_fold :: "('a \<times> 'b \<Rightarrow> 'c \<Rightarrow> 'c) \<Rightarrow> 'c \<Rightarrow> ('a \<rightharpoonup> 'b) \<Rightarrow> 'c" where
+  "\<not> finite (dom m) \<Longrightarrow> finite_map_fold f c m = undefined"
+| "finite (dom m) \<Longrightarrow> card (dom m) = 0 \<Longrightarrow> finite_map_fold f c m = c"
+| "finite (dom m) \<Longrightarrow> card (dom m) \<noteq> 0 \<Longrightarrow> finite_map_fold f c m = (
+    let x = SOME x. x \<in> dom m
+    in f (x, the (m x)) (finite_map_fold f c (m(x := None))))"
   by atomize_elim auto
 termination
-  proof (relation "measure (card o dom)")
-    show "wf (measure (card \<circ> dom))" by simp
+  proof (relation "measure (card o dom o snd o snd)")
+    show "wf (measure (card \<circ> dom o snd o snd))" by simp
   next
-    fix f :: "'a \<rightharpoonup> 'b"
+    fix f :: "'a \<times> 'b \<Rightarrow> 'c \<Rightarrow> 'c"
+    fix m :: "'a \<rightharpoonup> 'b"
+    fix c :: 'c 
     fix x
-    assume "card (dom f) \<noteq> 0"
-    then obtain y where "y \<in> dom f" by fastforce
-    hence "\<exists>y. y \<in> dom f" by fastforce
-    moreover assume "finite (dom f)"
-    moreover assume "x = (SOME x. x \<in> dom f)"
-    ultimately have "card (dom f - {x}) < card (dom f)" by (metis card_Diff1_less someI_ex)
-    thus "(f(x := None), f) \<in> measure (card \<circ> dom)" by simp
+    assume "card (dom m) \<noteq> 0"
+    then obtain y where "y \<in> dom m" by fastforce
+    hence "\<exists>y. y \<in> dom m" by fastforce
+    moreover assume "finite (dom m)"
+    moreover assume "x = (SOME x. x \<in> dom m)"
+    ultimately have "card (dom m - {x}) < card (dom m)" by (metis card_Diff1_less someI_ex)
+    thus "((f, c, m(x := None)), f, c, m) \<in> measure (card \<circ> dom o snd o snd)" by simp
   qed
 
-lemma [simp]: "finite (dom f) \<Longrightarrow> lookup (linearize f) x = f x"
-  proof (induction f rule: linearize.induct)
+definition linearize :: "('a \<rightharpoonup> 'b) \<Rightarrow> 'a \<leadsto> 'b" where
+  "linearize f = finite_map_fold (op #) [] f"
+
+lemma [simp]: "finite (dom f) \<Longrightarrow> lookup (finite_map_fold (op #) [] f) x = f x"
+  proof (induction "(op #)::('a \<times> 'b) \<Rightarrow> 'a \<leadsto> 'b \<Rightarrow> 'a \<leadsto> 'b" "[]::'a \<leadsto> 'b" f 
+         rule: finite_map_fold.induct)
   case 1
     thus ?case by simp
   next case 2
@@ -46,25 +52,33 @@ lemma [simp]: "finite (dom f) \<Longrightarrow> lookup (linearize f) x = f x"
       proof (cases "x = ?x")
       case True
         from 3 have "Some (the (f ?x)) = f ?x" 
-          by (metis (mono_tags, lifting) domIff fun_upd_triv linearize.simps(3) 
+          by (metis (mono_tags, lifting) domIff fun_upd_triv finite_map_fold.simps(3) 
               not_Cons_self2 option.collapse someI_ex)
         with 3 True show ?thesis by (simp add: Let_def)
       next case False
-        from 3 have "lookup (linearize (f(?x := None))) x = (f(?x := None)) x" by fastforce
+        from 3 have "lookup (finite_map_fold (op #) [] (f(?x := None))) x = (f(?x := None)) x" 
+          by fastforce
         with 3 False show ?thesis by (simp add: Let_def)
       qed
   qed
 
-lemma [simp]: "finite (dom f) \<Longrightarrow> domain_distinct (linearize f)"
-  proof (induction f rule: linearize.induct)
+lemma [simp]: "finite (dom f) \<Longrightarrow> lookup (linearize f) x = f x"
+  by (simp add: linearize_def)
+
+lemma [simp]: "finite (dom f) \<Longrightarrow> domain_distinct (finite_map_fold (op #) [] f)"
+  proof (induction "(op #)::('a \<times> 'b) \<Rightarrow> 'a \<leadsto> 'b \<Rightarrow> 'a \<leadsto> 'b" "[]::'a \<leadsto> 'b" f 
+         rule: finite_map_fold.induct)
   case 1
     thus ?case by simp
   next case 2
     thus ?case by simp
   next case (3 f)
     let ?x = "SOME x. x \<in> dom f"
-    from 3 have "domain_distinct (linearize (f(?x := None)))" by fastforce
+    from 3 have "domain_distinct (finite_map_fold (op #) [] (f(?x := None)))" by fastforce
     with 3 show ?case by (auto simp add: Let_def)
   qed
+
+lemma [simp]: "finite (dom f) \<Longrightarrow> domain_distinct (linearize f)"
+  by (simp add: linearize_def)
 
 end
